eve/Src/examples/proofs/invalid_frames/if_client.e
@@ -1,0 +1,54 @@
+indexing
+	description: "Summary description for {IF_CLIENT}."
+	date: "$Date$"
+	revision: "$Revision$"
+
+class
+	IF_CLIENT
+
+create
+	make
+
+feature
+
+	make
+		local
+			p: IF_PARENT
+			c: IF_CHILD
+		do
+			create p.make
+			create c.make
+
+			check
+				p.field1 = 1
+				p.field2 = 2
+				c.field1 = 1
+				c.field2 = 2
+			end
+
+			p.foo (4)
+
+			check
+				p.field1 = 4
+				p.field2 = 2
+				c.field1 = 1
+				c.field2 = 2
+			end
+
+			p := c
+
+			check
+				p.field1 = 1
+				p.field2 = 2
+			end
+
+			p.foo (4)
+
+			check
+				p.field1 = 4
+				wrong: p.field2 = 2		-- p.field2 is actually 5
+			end
+
+		end
+
+end
