eve/Src/examples/proofs/invalid_frames/if_parent.e
@@ -1,0 +1,38 @@
+indexing
+	description: "Summary description for {IF_PARENT}."
+	date: "$Date$"
+	revision: "$Revision$"
+
+class
+	IF_PARENT
+
+create
+	make
+
+feature {NONE} -- Initialization
+
+	make
+		do
+			field1 := 1
+			field2 := 2
+		ensure
+			field1 = 1
+			field2 = 2
+		end
+
+feature -- Access
+
+	field1: INTEGER
+
+	field2: INTEGER
+
+feature -- Element change
+
+	foo (arg: INTEGER)
+		do
+			field1 := arg
+		ensure
+			field1 = arg
+		end
+
+end
