eve/Src/framework/eve_proofs/error/ep_frame_error.e
@@ -1,0 +1,29 @@
+indexing
+	description:
+		"[
+			TODO
+		]"
+	date: "$Date$"
+	revision: "$Revision$"
+
+class EP_FRAME_ERROR
+
+inherit
+	EP_ERROR
+		rename
+			make as make_with_message
+		end
+
+create
+	make
+
+feature {NONE} -- Initialization
+
+	make
+			-- Initialize frame error.
+		do
+			make_with_message (names.error_frame_violation)
+			set_description (names.description_frame_violation)
+		end
+
+end
